re-adding spec to env translation

props.lean
@@ -10,6 +10,17 @@ inductive free_in_term (x: var) : term → Prop
 | app₁ {t₁ t₂: term}               : free_in_term t₁ → free_in_term (term.app t₁ t₂)
 | app₂ {t₁ t₂: term}               : free_in_term t₂ → free_in_term (term.app t₁ t₂)
 
+inductive free_in_spec (x: var) : spec → Prop
+| term {t: term}                       : free_in_term x t → free_in_spec (spec.term t)
+| not {R: spec}                        : free_in_spec R  → free_in_spec (spec.not R)
+| and₁ {R S: spec}                     : free_in_spec R → free_in_spec (spec.and R S)
+| and₂ {R S: spec}                     : free_in_spec S → free_in_spec (spec.and R S)
+| or₁ {R S: spec}                      : free_in_spec R → free_in_spec (spec.or R S)
+| or₂ {R S: spec}                      : free_in_spec S → free_in_spec (spec.or R S)
+| func₁ {y: var} {t: term} {R S: spec} : (x ≠ y) → free_in_term x t → free_in_spec (spec.func t y R S)
+| func₂ {y: var} {t: term} {R S: spec} : (x ≠ y) → free_in_spec R → free_in_spec (spec.func t y R S)
+| func₃ {y: var} {t: term} {R S: spec} : (x ≠ y) → free_in_spec S → free_in_spec (spec.func t y R S)
+
 inductive free_in_prop (x: var) : prop → Prop
 | term {t: term}                        : free_in_term x t → free_in_prop t
 | not {p: prop}                         : free_in_prop p → free_in_prop (prop.not p)
@@ -30,11 +41,24 @@ inductive free_in_prop (x: var) : prop → Prop
 | forallc₂ {y: var} {t: term} {p: prop} : (x ≠ y) → free_in_prop p → free_in_prop (prop.forallc y t p)
 | exist {y: var} {p: prop}              : (x ≠ y) → free_in_prop p → free_in_prop (prop.exist y p)
 
--- notation x ∈ FV p
+-- notation x ∈ FV t/p
 
-structure freevars := (p: prop)
-instance : has_mem var freevars := ⟨λx fv, free_in_prop x fv.p⟩ 
-def FV(p: prop): freevars := freevars.mk p
+inductive freevars
+| term: term → freevars
+| spec: spec → freevars
+| prop: prop → freevars
+
+class has_fv (α: Type) := (fv : α → freevars)
+instance : has_fv term := ⟨freevars.term⟩
+instance : has_fv spec := ⟨freevars.spec⟩
+instance : has_fv prop := ⟨freevars.prop⟩
+
+def freevars.to_set: freevars → set var
+| (freevars.term t) := λx, free_in_term x t
+| (freevars.spec R) := λx, free_in_spec x R
+| (freevars.prop P) := λx, free_in_prop x P
+
+def FV {α: Type} [h: has_fv α] (a: α): set var := (has_fv.fv a).to_set
 
 -- helper lemmas
 
@@ -170,11 +194,3 @@ lemma call_history_closed (H: list call) (x: var): ¬ free_in_prop x (calls_to_p
       )
     )
   )
-
--- validity
-
-inductive valid : prop → Prop
-notation `⟪` p `⟫`: 100 := valid p
-| to_prop {p: prop}: valid p
-
-notation `⟪` p `⟫`: 100 := valid p
