logic.lean
@@ -1,0 +1,147 @@
+import .syntax .etc .props
+
+-- instantiation
+
+constant prop.instantiated: prop → qfprop → Prop
+
+-- substitution
+
+inductive term.substituted (x: var) (v: value): term → term → Prop
+
+| value {v': value} :
+    term.substituted v' v'
+
+| same_var:
+    term.substituted x v
+
+| diff_var {y: var}:
+    (x ≠ y) →
+    term.substituted y y
+
+| unop {op: unop} {t t': term}:
+    term.substituted t t' →
+    term.substituted (term.unop op t) (term.unop op t')
+
+| binop {op: binop} {t₁ t₂ t₁' t₂': term}:
+    term.substituted t₁ t₁' →
+    term.substituted t₂ t₂' →
+    term.substituted (term.binop op t₁ t₂) (term.binop op t₁' t₂')
+
+| app {t₁ t₂ t₁' t₂': term}:
+    term.substituted t₁ t₁' →
+    term.substituted t₂ t₂' →
+    term.substituted (term.app t₁ t₂) (term.app t₁' t₂')
+
+inductive spec.substituted (x: var) (v: value): spec → spec → Prop
+
+| term {t t': term} :
+    term.substituted x v t t' →
+    spec.substituted (spec.term t) (spec.term t')
+
+| not {R R': spec} :
+    spec.substituted R R' →
+    spec.substituted (spec.not R) (spec.not R')
+
+| and {R S R' S': spec} :
+    spec.substituted R R' →
+    spec.substituted S S' →
+    spec.substituted (spec.and R S) (spec.and R' S')
+
+| or {R S R' S': spec} :
+    spec.substituted R R' →
+    spec.substituted S S' →
+    spec.substituted (spec.or R S) (spec.or R' S')
+
+| func_same {R S: spec} {t t': term} :
+    term.substituted x v t t' →
+    spec.substituted (spec.func t x R S) (spec.func t' x R S)
+
+| func {y: var} {R S R' S': spec} {t t': term} :
+    (x ≠ y) →
+    term.substituted x v t t' →
+    spec.substituted R R' →
+    spec.substituted S S' →
+    spec.substituted (spec.func t y R S) (spec.func t' y R' S')
+
+inductive spec.substituted_env: env → spec → spec → Prop
+
+| empty {R: spec}:
+    spec.substituted_env env.empty R R
+
+| cons {σ: env} {x: var} {v: value} {R R' R'': spec} :
+    spec.substituted x v R R' →
+    spec.substituted_env σ R' R'' →
+    spec.substituted_env (σ[x↦v]) R R''
+
+inductive qfprop.substituted (x: var) (v: value): qfprop → qfprop → Prop
+
+| term {t t': term} :
+    term.substituted x v t t' →
+    qfprop.substituted (qfprop.term t) (qfprop.term t')
+
+| not {P P': qfprop} :
+    qfprop.substituted P P' →
+    qfprop.substituted (qfprop.not P) (qfprop.not P')
+
+| and {P Q P' Q': qfprop} :
+    qfprop.substituted P P' →
+    qfprop.substituted Q Q' →
+    qfprop.substituted (qfprop.and P Q) (qfprop.and P' Q')
+
+| or {P Q P' Q': qfprop} :
+    qfprop.substituted P P' →
+    qfprop.substituted Q Q' →
+    qfprop.substituted (qfprop.or P Q) (qfprop.or P' Q')
+
+| pre {t₁ t₂ t₁' t₂': term}:
+    term.substituted x v t₁ t₁' →
+    term.substituted x v t₂ t₂' →
+    qfprop.substituted (qfprop.pre t₁ t₂) (qfprop.pre t₁' t₂')
+
+| pre₁ {op: unop} {t t': term} :
+    term.substituted x v t t' →
+    qfprop.substituted (qfprop.pre₁ op t) (qfprop.pre₁ op t')
+
+| pre₂ {op: binop} {t₁ t₂ t₁' t₂': term}:
+    term.substituted x v t₁ t₁' →
+    term.substituted x v t₂ t₂' →
+    qfprop.substituted (qfprop.pre₂ op t₁ t₂) (qfprop.pre₂ op t₁' t₂')
+
+| post {t₁ t₂ t₁' t₂': term}:
+    term.substituted x v t₁ t₁' →
+    term.substituted x v t₂ t₂' →
+    qfprop.substituted (qfprop.post t₁ t₂) (qfprop.post t₁' t₂')
+
+inductive qfprop.substituted_env: env → qfprop → qfprop → Prop
+
+| empty {P: qfprop}:
+    qfprop.substituted_env env.empty P P
+
+| cons {σ: env} {x: var} {v: value} {P P' P'': qfprop} :
+    qfprop.substituted x v P P' →
+    qfprop.substituted_env σ P' P'' →
+    qfprop.substituted_env (σ[x↦v]) P P''
+
+-- validity
+
+inductive valid : qfprop → Prop
+notation `⊨` p: 100 := valid p
+
+| tru: ⊨ value.true
+
+| eq {t: term}: ⊨ term.binop binop.eq t t
+
+| and {q p: qfprop}: ⊨ p → ⊨ q → ⊨ (p & q)
+
+| orl {q p: qfprop}: ⊨ p → ⊨ (qfprop.or p q)
+
+| orr {q p: qfprop}: ⊨ q → ⊨ (qfprop.or p q)
+
+| mp {q p: qfprop}: ⊨ qfprop.implies p q → ⊨ p → ⊨ q
+
+notation `⊨` p: 100 := valid p
+
+@[reducible]
+def VC(P: prop) := ∀ (σ: env) (P' P'': qfprop), (prop.instantiated P P') → (qfprop.substituted_env σ P' P'') → ⊨ P''
+
+notation `⟪` P `⟫`: 100 := VC P
