vcgen.lean
@@ -1,4 +1,4 @@
-import .syntax .etc .evaluation .props
+import .syntax .etc .evaluation .props .logic
 
 reserve infix `⊢`:10
 
@@ -23,6 +23,8 @@ notation P `⊢` e `:` Q : 10 := exp.vcgen P e Q
 | func {P: prop} {f x: var} {R S: spec} {e₁ e₂: exp} {Q₁ Q₂: propctx}:
     f ∉ FV P →
     x ∉ FV P →
+    FV P ⊇ FV R →
+    FV P ⊇ FV S →
     (P & spec.func f x R S & R ⊢ e₂ : Q₂) →
     ⟪prop.implies (P & spec.func f x R S & R & Q₂ (term.app f x)) S⟫ →
     (P ⊢ letf f[x] req R ens S {e₁} in e₂ :
@@ -82,12 +84,17 @@ notation `⊢` σ `:` Q : 10 := env.vcgen σ Q
     (⊢ σ : Q) →
     (⊢ (σ[x ↦ value.num n]) : (Q & x ≡ value.num n))
 
-| func {σ₁ σ₂: env} {f g x: var} {R S: spec} {e: exp} {Q₁ Q₂: prop} {Q₃: propctx}:
+| func {σ₁ σ₂: env} {f g x: var} {R R' S S': spec} {e: exp} {Q₁ Q₂: prop} {Q₃: propctx}:
     (⊢ σ₁ : Q₁) →
     (⊢ σ₂ : Q₂) →
+    FV Q₂ ∪ { g, x } ⊇ FV R →
+    FV Q₂ ∪ { g, x } ⊇ FV S →
+    spec.substituted_env (σ₂[g↦value.func g x R S e σ₂]) R R' →
+    spec.substituted_env (σ₂[g↦value.func g x R S e σ₂]) S S' →
     (Q₂ & spec.func g x R S & R ⊢ e : Q₃) →
     ⟪prop.implies (Q₂ & spec.func g x R S & R & Q₃ (term.app g x)) S⟫ →
-    (⊢ (σ₁[f ↦ value.func g x R S e σ₂]) : (Q₁ & spec.func f x R S & f ≡ value.func g x R S e σ₂))
+    (⊢ (σ₁[f ↦ value.func g x R S e σ₂]) :
+      (Q₁ & spec.func f x R' S' & f ≡ value.func g x R S e σ₂))
 
 notation `⊢` σ `:` Q : 10 := env.vcgen σ Q
 
